src/Promising.v
@@ -209,7 +209,7 @@ Section FwdItem.
   Hint Constructors t.
 
   Definition read_view (fwd:t) (tsx:Time.t) (ord:OrdR.t): View.t (A:=A) :=
-    if andb (fwd.(ts) == tsx) (orb (negb fwd.(ex)) (negb (OrdR.ge ord OrdR.acquire_pc)))
+    if andb (fwd.(ts) == tsx) (negb (andb fwd.(ex) (orb (arch == riscv) (OrdR.ge ord OrdR.acquire_pc))))
     then fwd.(view)
     else View.mk tsx bot.
 End FwdItem.
